agtTypes.v
@@ -1,0 +1,7 @@
+
+Inductive primitive_type : Set :=
+| Int : primitive_type
+| Bool : primitive_type.
+Definition primitive_type_dec : ∀ n m : primitive_type, {n = m} + {n ≠ m}. decide equality. Defined.
+Program Instance primitive_type_EqDec : EqDec primitive_type eq := primitive_type_dec.
+Hint Resolve primitive_type_dec.
